WIP FTLR switcher return

theories/ftlr/ftlr_switcher_return.v
@@ -31,6 +31,102 @@ Section fundamental.
   Implicit Types w : (leibnizO Word).
   Implicit Types interp : (V).
 
+
+  Lemma region_open_list_interp_gen (W : WORLD) (C : CmptName)
+    (la la' : list Addr) (p : Perm) (g : Locality) (b e a : Addr) :
+    NoDup la ->
+    readAllowed p = true →
+    Forall (fun a' : Addr => (b <= a' < e)%a ) la ->
+    la ## la' ->
+
+    interp W C (WCap p g b e a)
+    ∗ open_region_many W C la'
+    ∗ sts_full_world W C -∗
+
+    ∃ (l : list (Word * Perm * (WORLD * CmptName * Word → iProp Σ) * region_type)),
+      open_region_many W C (la++la')
+      ∗ sts_full_world W C
+      ∗ ([∗ list] a ; '(v,p,φ,ρ) ∈ la ; l, sts_state_std C a ρ)
+      ∗ ([∗ list] a ; '(v,p,φ,ρ) ∈ la ; l, a ↦ₐ v)
+      ∗ ▷ ([∗ list] '(v,p,φ,ρ) ∈ l, monotonicity_guarantees_region C φ p v ρ)
+      ∗ ▷ ([∗ list] '(v,p,φ,ρ) ∈ l, φ (W, C, v))
+      ∗ ▷ ([∗ list] '(v,p,φ,ρ) ∈ l, rcond (safeUC φ) C p interp)
+      ∗ ([∗ list] a ; '(v,p,φ,ρ) ∈ la ; l, rel C a p φ)
+      ∗ ⌜ length l = length la ⌝
+  .
+  Proof.
+    induction la; intros Hnodup Hp Hin Hdis ;
+      iIntros "(#Hinterp & Hr & Hsts)"; cbn in * |- *.
+    - iExists []; cbn in *.
+      by iFrame.
+    - apply Forall_cons in Hin; destruct Hin as [Hin_a0 Hin].
+      apply list.NoDup_cons in Hnodup; destruct Hnodup as [Hnotin Hnodup].
+      pose proof (disjoint_cons _ _ _ Hdis) as Ha_notin_l'.
+      eapply disjoint_weak in Hdis.
+      iDestruct (IHla with "[$Hinterp $Hr $Hsts]") as "IH"; eauto.
+      iDestruct "IH" as (lv) "(Hr & Hsts & Hsts_stds & Hlv & Hmono & Hlφ & Hrcond & Hrel & %Hlen)".
+      iDestruct (read_allowed_inv _ _ a0 with "Hinterp")
+        as (p' P) "(%Hperm_flow & %Hpers_P & Hrel_P & Hzcond_P & Hrcond_P & Hwcond_P & HmonoV)"
+      ; auto.
+      iDestruct (readAllowed_valid_cap_implies with "Hinterp") as (ρ) "[%HWa %Hρ]"; auto.
+      { by eapply withinBounds_true_iff. }
+      iDestruct (region_open_next with "[$Hr $Hrel_P $Hsts]") as "Ha"; eauto.
+      {
+        intros Hcontra.
+        apply elem_of_app in Hcontra. destruct Hcontra as [Hcontra|Hcontra]
+        ; [set_solver+Hcontra Hnotin|set_solver+Hcontra Ha_notin_l'].
+      }
+      iDestruct "Ha" as (va) "(Hsts & Hsts_std_a & Hr & Hv_a & Hmono_a & Hφ_a & %Hp_a)".
+      iExists ((va, p', safeC P, ρ)::lv).
+      iFrame "∗#".
+      iPureIntro ; cbn ; lia.
+  Qed.
+
+  Lemma region_open_list_interp (W : WORLD) (C : CmptName)
+    (la' : list Addr) (p : Perm) (g : Locality) (b e a : Addr) :
+    let la := finz.seq_between b e in
+    readAllowed p = true →
+    la ## la' ->
+
+    interp W C (WCap p g b e a)
+    ∗ open_region_many W C la'
+    ∗ sts_full_world W C -∗
+
+    ∃ (l : list (Word * Perm * (WORLD * CmptName * Word → iProp Σ) * region_type)),
+      open_region_many W C (la++la')
+      ∗ sts_full_world W C
+      ∗ ([∗ list] a ; '(v,p,φ,ρ) ∈ la ; l, sts_state_std C a ρ)
+      ∗ ([∗ list] a ; '(v,p,φ,ρ) ∈ la ; l, a ↦ₐ v)
+      ∗ ▷ ([∗ list] '(v,p,φ,ρ) ∈ l, monotonicity_guarantees_region C φ p v ρ)
+      ∗ ▷ ([∗ list] '(v,p,φ,ρ) ∈ l, φ (W,C,v))
+      ∗ ▷ ([∗ list] '(v,p,φ,ρ) ∈ l, rcond (safeUC φ) C p interp)
+      ∗ ([∗ list] a ; '(v,p,φ,ρ) ∈ la ; l, rel C a p φ)
+      ∗ ⌜ length l = length la ⌝
+  .
+  Proof.
+    iIntros (la Hp Hdis).
+    iApply region_open_list_interp_gen; eauto; subst la.
+    - apply finz_seq_between_NoDup.
+    - apply Forall_forall ; intros.
+      by apply elem_of_finz_seq_between.
+  Qed.
+
+  Definition closing_resources W C a w : iProp Σ :=
+    ∃ φ p ρ,
+      (sts_state_std C a ρ
+       ∗ (φ (W, C, w))
+       ∗ (monotonicity_guarantees_region C φ p w ρ)
+       ∗ rcond (safeUC φ) C p interp
+       ∗ rel C a p φ)%I.
+
+  Lemma closing_resources_interp W C a w :
+    closing_resources W C a w -∗ interp W C w.
+    iIntros "H".
+    iDestruct "H" as (???) "(Hstd&Hφ&Hmono&Hrcond&Hrel)".
+    destruct p.
+    destruct dl,dro; by iApply "Hrcond".
+  Qed.
+
   Lemma switcher_return_ftlr (W : WORLD) (C : CmptName) (rmap : leibnizO Reg)
     (cstk : CSTK) (wstk : Word)
     (Nswitcher : namespace)
@@ -170,42 +266,72 @@ Section fundamental.
     destruct HWF as (Hb_a4 & He_a1 & [a_stk4 Ha_stk4]).
 
     iDestruct "Hcont_K" as "(Hcont_K & #Hinterp_callee_wstk & Hexec_topmost_frm)".
-    (* TODO: be clever to not repeat the proof,
-       and assert
-       (exists wa4,
-       (if is_untrusted_caller then V(wa4) else ⌜wa4 = wcs2⌝ ) ∗
-       (a_stk ^+ -4 ↦ₐ wa4)
-       )
-       etc
-     *)
+    iEval (cbn) in "Hinterp_callee_wstk".
+    iDestruct (lc_fupd_elim_later with "[$] [$Hinterp_callee_wstk]") as ">#Hinterp_callee_wstk'".
+    iClear "Hinterp_callee_wstk" ; iRename "Hinterp_callee_wstk'" into "Hinterp_callee_wstk".
 
     iAssert (
-        |={⊤}=>
         ∃ wastk wastk1 wastk2 wastk3,
           a_stk ↦ₐ wastk
           ∗ (a_stk ^+ 1)%a ↦ₐ wastk1
           ∗ (a_stk ^+ 2)%a ↦ₐ wastk2
           ∗ (a_stk ^+ 3)%a ↦ₐ wastk3
           ∗ (if is_untrusted_caller
-             then (interp W C wastk ∗ interp W C wastk1 ∗ interp W C wastk2 ∗ interp W C wastk3)
+             then
+               ▷ (closing_resources W C a_stk wastk
+               ∗ closing_resources W C (a_stk ^+ 1)%a wastk1
+               ∗ closing_resources W C (a_stk ^+ 2)%a wastk2
+               ∗ closing_resources W C (a_stk ^+ 3)%a wastk3)
              else (⌜ wastk = wcs2 ⌝ ∗ ⌜ wastk1 = wcs3 ⌝ ∗ ⌜ wastk2 = wret ⌝ ∗ ⌜ wastk3 = wcgp0 ⌝)
             )
+          ∗ open_region_many W C (if is_untrusted_caller then [a_stk;(a_stk ^+ 1)%a;(a_stk ^+ 2)%a;(a_stk ^+ 3)%a] else [])
+          ∗ sts_full_world W C
       )%I
-       with "[Hcframe_interp Hlc]" as ">Hcframe_interp"
+      with "[Hcframe_interp Hr Hsts]" as "Hcframe_interp"
     ; [|iDestruct "Hcframe_interp" as
-        (wastk wastk1 wastk2 wastk3) "(Ha_stk & Ha_stk1 & Ha_stk2 & Ha_stk3 & Hwstk)"
+        (wastk wastk1 wastk2 wastk3) "(Ha_stk & Ha_stk1 & Ha_stk2 & Ha_stk3 & Hwstk & Hr & Hsts)"
       ].
     {
       destruct is_untrusted_caller; cycle 1.
-      * iModIntro.
-        iExists wcs2, wcs3, wret, wcgp0.
+      * iExists wcs2, wcs3, wret, wcgp0.
+        rewrite region_open_nil; iFrame "Hr Hsts".
         by iDestruct "Hcframe_interp" as "($&$&$&$)".
-      * iDestruct (lc_fupd_elim_later with "[$] [$Hinterp_callee_wstk]") as ">#Hinterp_callee_wstk'"; iModIntro.
-        iClear "Hinterp_callee_wstk" ; iRename "Hinterp_callee_wstk'" into "Hinterp_callee_wstk".
-        iEval (cbn) in "Hinterp_callee_wstk".
-        admit. (* we probably need to open the region *)
+      * rewrite region_open_nil.
+
+
+        iDestruct (region_open_list_interp_gen _ _ (finz.seq_between a_stk (a_stk^+4)%a)
+                    with "[$Hinterp_callee_wstk $Hr $Hsts]")
+          as (l) "(Hr & Hsts & Hstd & Hv & Hmono & Hφ & Hrcond & Hrel & %Hlen_l)"; auto.
+        { eapply finz_seq_between_NoDup. }
+        { clear-He_a1 ; apply Forall_forall; intros a' Ha'.
+          apply elem_of_finz_seq_between in Ha'; solve_addr.
+        }
+        { set_solver. }
+        cbn in Hlen_l.
+        do 4 (rewrite finz_seq_between_cons in Hlen_l; last solve_addr+He_a1).
+        rewrite finz_seq_between_empty in Hlen_l; last solve_addr+.
+        cbn in Hlen_l.
+        destruct l as [| [ [ [wastk0 p0] φ0] ρ0] l]; first (by cbn in Hlen_l).
+        destruct l as [| [ [ [wastk1 p1] φ1] ρ1] l]; first (by cbn in Hlen_l).
+        destruct l as [| [ [ [wastk2 p2] φ2] ρ2] l]; first (by cbn in Hlen_l).
+        destruct l as [| [ [ [wastk3 p3] φ3] ρ3] l]; first (by cbn in Hlen_l).
+        destruct l as [|]; last (by cbn in Hlen_l).
+        do 4 (rewrite (finz_seq_between_cons _ (a_stk ^+ 4)%a); last solve_addr+He_a1).
+        rewrite (finz_seq_between_empty _ (a_stk ^+ 4)%a); last solve_addr+.
+        cbn.
+        replace ((a_stk ^+ 1) ^+ 1)%a with (a_stk ^+ 2)%a by solve_addr+Ha_stk4.
+        replace ((a_stk ^+ 2) ^+ 1)%a with (a_stk ^+ 3)%a by solve_addr+Ha_stk4.
+        iDestruct "Hv" as "($&$&$&$&_)".
+        iFrame.
+        iDestruct "Hrcond" as "(Hrcond_0 & Hrcond_1 & Hrcond_2 & Hrcond_3 & _)".
+        iDestruct "Hrel" as "(Hrel_0 & Hrel_1 & Hrel_2 & Hrel_3 & _)".
+        iDestruct "Hφ" as "(Hφ_0 & Hφ_1 & Hφ_2 & Hφ_3 & _)".
+        iDestruct "Hmono" as "(Hmono_0 & Hmono_1 & Hmono_2 & Hmono_3 & _)".
+        iDestruct "Hstd" as "(Hstd_0 & Hstd_1 & Hstd_2 & Hstd_3 & _)".
+        rewrite /closing_resources.
+        iFrame.
     }
-    (* iDestruct "Hcframe_interp" as "(Ha_stk & Ha_stk1 & Ha_stk2 & Ha_stk3)". *)
+
     destruct (decide (a_tstk < e_trusted_stack)%a) as [Htstk_ae|Htstk_ae]; cycle 1.
     { admit. (* NOTE will fail in the next upcoming instructions *) }
     (* Load csp ctp *)
@@ -213,38 +339,6 @@ Section fundamental.
     { split ; [ solve_pure | rewrite le_addr_withinBounds ; solve_addr ]. }
     rewrite -/(interp_cont).
     iEval (cbn) in "Hinterp_callee_wstk".
-
-    (* assert (is_Some (a_stk4 + -1)%a) as [a_stk3 Ha_stk3] by solve_addr+Ha_stk4. *)
-    (* replace (a_stk4 ^+ -1)%a with a_stk3 by solve_addr+Ha_stk3. *)
-    (* replace (a_stk ^+ 3)%a with a_stk3. *)
-    (* 2: { clear -Ha_stk4 Ha_stk3. *)
-    (*      assert ( a_stk4 = a_stk ^+ 4 )%a by solve_addr. *)
-    (*      rewrite H in Ha_stk3. *)
-    (*      replace ( (a_stk ^+ 4 + -1)%a) with ( (a_stk + 3)%a); solve_addr. *)
-    (* } *)
-
-    (* assert (is_Some (a_stk4 + -2)%a) as [a_stk2 Ha_stk2] by solve_addr+Ha_stk4. *)
-    (* replace (a_stk4 ^+ -2)%a with a_stk2 by solve_addr+Ha_stk2. *)
-    (* replace (a_stk ^+ 2)%a with a_stk2. *)
-    (* 2: { clear -Ha_stk4 Ha_stk2. *)
-    (*      assert ( a_stk4 = a_stk ^+ 4 )%a by solve_addr. *)
-    (*      rewrite H in Ha_stk2. *)
-    (*      replace ( (a_stk ^+ 4 + -2)%a) with ( (a_stk + 2)%a); solve_addr. *)
-    (* } *)
-
-    (* assert (is_Some (a_stk4 + -3)%a) as [a_stk1 Ha_stk1] by solve_addr+Ha_stk4. *)
-    (* replace (a_stk4 ^+ -3)%a with a_stk1 by solve_addr+Ha_stk1. *)
-    (* replace (a_stk ^+ 1)%a with a_stk1. *)
-    (* 2: { clear -Ha_stk4 Ha_stk1. *)
-    (*      assert ( a_stk4 = a_stk ^+ 4 )%a by solve_addr. *)
-    (*      rewrite H in Ha_stk1. *)
-    (*      replace ( (a_stk ^+ 4 + -3)%a) with ( (a_stk + 1)%a); solve_addr. *)
-    (* } *)
-
-    (* replace (a_stk4 ^+ -4)%a with a_stk by solve_addr+Ha_stk4. *)
-    (* replace (a_stk ^+ 4)%a with a_stk4 by solve_addr+Ha_stk4. *)
-
-
 
     (* Lea ctp (-1)%Z *)
     iInstr "Hcode".
@@ -286,38 +380,31 @@ Section fundamental.
     unfocus_block "Hcode" "Hcont" as "Hcode"; subst hcont.
 
 
-    set ( callee_stk_range := (finz.seq_between (a_stk ^+4)%a e_stk ) ).
-    assert (Forall (fun a => (std W) !! a = Some Temporary) callee_stk_range)
-      as Hcallee_stk_temporary.
-    { (* I should get this from Hinterp_callee_wstk *)
-      admit.
-      (* apply Forall_forall. *)
-      (* intros a Ha. *)
-      (* eapply region_state_pub_temp; eauto. *)
-      (* subst W1. *)
-      (* cbn. *)
-      (* destruct (decide (a ∈ a_local_args)). *)
-      (* - by apply std_sta_update_multiple_lookup_in_i. *)
-      (* - rewrite std_sta_update_multiple_lookup_same_i; last done. *)
-      (*   rewrite frame_W_lookup_std. *)
-      (*   by apply std_sta_update_multiple_lookup_in_i. *)
-    }
 
-    iAssert ([∗ list] a ∈ callee_stk_range, rel C a RWL interpC)%I as "Hrel_stk_callee".
+    iDestruct (region_open_list_interp_gen _ _ (finz.seq_between (a_stk^+4)%a e_stk)
+                with "[$Hinterp_callee_wstk $Hr $Hsts]")
+      as (l) "(Hr & Hsts & Hstd & Hv & Hmono & Hφ & Hrcond & Hrel & %Hlen_l)"; auto.
+    { eapply finz_seq_between_NoDup. }
+    { clear-He_a1 ; apply Forall_forall; intros a' Ha'.
+      apply elem_of_finz_seq_between in Ha'.
+      destruct is_untrusted_caller; solve_addr.
+    }
     {
-      (* iDestruct (read_allowed_inv with "Hinterp_callee_wstk") as "H". *)
-      admit.
+      destruct is_untrusted_caller; last set_solver.
+      set (la := finz.seq_between (a_stk ^+ 4)%a e_stk).
+      assert ( a_stk ∉ la) by (subst la; apply not_elem_of_finz_seq_between; solve_addr+).
+      assert ( (a_stk ^+ 1)%a ∉ la) by (subst la; apply not_elem_of_finz_seq_between; solve_addr+).
+      assert ( (a_stk ^+ 2)%a ∉ la) by (subst la; apply not_elem_of_finz_seq_between; solve_addr+).
+      assert ( (a_stk ^+ 3)%a ∉ la) by (subst la; apply not_elem_of_finz_seq_between; solve_addr+).
+      set_solver.
     }
-    iDestruct (region_open_list_alt with "[$Hrel_stk_callee $Hr $Hsts]") as (lv) "(Hr & Hsts & Hstd & Hstk & Hmono & Hφ)"
-    ; eauto.
-    { apply finz_seq_between_NoDup. }
-    { auto. }
-
+    set (lv := map (fun x => let '(v, _, _, _) := x in v) l).
 
     iAssert ([[ a_stk , e_stk ]] ↦ₐ [[wastk :: wastk1 :: wastk2 :: wastk3 :: lv]])%I
-      with "[Ha_stk Ha_stk1 Ha_stk2 Ha_stk3 Hstk]" as "Hstk".
+      with "[Ha_stk Ha_stk1 Ha_stk2 Ha_stk3 Hv]" as "Hstk".
     {
-      iAssert ([[ (a_stk ^+ 4)%a , e_stk ]] ↦ₐ [[ lv ]])%I with "[$Hstk]" as "Hstk".
+      iAssert ([[ (a_stk ^+ 4)%a , e_stk ]] ↦ₐ [[ lv ]])%I with "[Hv]" as "Hstk".
+      { admit. (* should be fairly easy, just projections *) }
       iDestruct (region_pointsto_cons with "[$Ha_stk3 $Hstk]") as "Hstk"; [solve_addr+Ha_stk4|solve_addr+He_a1|].
       iDestruct (region_pointsto_cons with "[$Ha_stk2 $Hstk]") as "Hstk"; [solve_addr+Ha_stk4|solve_addr+He_a1|].
       iDestruct (region_pointsto_cons with "[$Ha_stk1 $Hstk]") as "Hstk"; [solve_addr+Ha_stk4|solve_addr+He_a1|].
@@ -331,17 +418,13 @@ Section fundamental.
 
     focus_block 8 "Hcode" as a8 Ha8 "Hcode" "Hcont"; iHide "Hcont" as hcont.
     (* Mov cra ca2 *)
-    iInstr "Hcode".
+    iInstr "Hcode" with "Hlc".
     unfocus_block "Hcode" "Hcont" as "Hcode"; subst hcont.
 
     focus_block 9 "Hcode" as a9 Ha9 "Hcode" "Hcont"; iHide "Hcont" as hcont.
     iDestruct (big_sepM_insert_delete with "[$Hrmap $Hct1]") as "Hrmap".
     rewrite -delete_insert_ne //.
     iDestruct (big_sepM_insert_delete with "[$Hrmap $Hct0]") as "Hrmap".
-    (* do 2 (rewrite -delete_insert_ne //). *)
-    (* iDestruct (big_sepM_insert_delete with "[$Hrmap $Hcs0]") as "Hrmap". *)
-    (* do 3 (rewrite -delete_insert_ne //). *)
-    (* iDestruct (big_sepM_insert_delete with "[$Hrmap $Hcs1]") as "Hrmap". *)
     do 2 (rewrite (delete_commute _ _ ca2); auto).
     do 2 (rewrite -delete_insert_ne //).
     iDestruct (big_sepM_insert_delete with "[$Hrmap $Hca2]") as "Hrmap".
@@ -394,7 +477,7 @@ Section fundamental.
     rewrite /interp_cont_exec.
     iEval (cbn) in "Hexec_topmost_frm".
     iAssert ([∗ map] r↦w ∈ arg_rmap', r ↦ᵣ WInt 0)%I with "[Harg_rmap']" as "Hrmap".
-    { admit. }
+    { admit. (* easy *) }
 
     destruct is_untrusted_caller.
     - (* Case where caller is untrusted, we use the IH *)
@@ -408,7 +491,15 @@ Section fundamental.
             iApply wp_value; iIntros; discriminate.
       }
       (* The PC is correct, we can use the continuation*)
-      iDestruct "Hwstk" as "(#Hinterp_wcs2 & #Hinterp_wcs3 & #Hinterp_wret & #Hinterp_wcgp0)".
+      iDestruct "Hlc" as "[Hlc Hlc']".
+      iDestruct (lc_fupd_elim_later with "[$Hlc'] [$Hwstk]") as ">Hwstk".
+      iDestruct "Hwstk" as "(Hclose_wastk & Hclose_wastk1 & Hclose_wastk2 & Hclose_wastk3)".
+
+      iDestruct (closing_resources_interp with "Hclose_wastk") as "#Hinterp_wastk".
+      iDestruct (closing_resources_interp with "Hclose_wastk1") as "#Hinterp_wastk1".
+      iDestruct (closing_resources_interp with "Hclose_wastk2") as "#Hinterp_wastk2".
+      iDestruct (closing_resources_interp with "Hclose_wastk3") as "#Hinterp_wastk3".
+
       iAssert (
           ∃ rmap', ⌜ dom rmap' = dom arg_rmap' ⌝ ∗ ([∗ map] r↦w ∈ rmap', r ↦ᵣ w)
                    ∗ (∀ (r : RegName) (v : leibnizO Word), ⌜r ≠ PC⌝ → ⌜rmap' !! r = Some v⌝ → interp W C v)
@@ -416,7 +507,8 @@ Section fundamental.
       {
         iExists (fmap (fun v => WInt 0) arg_rmap').
         iSplit ; [iPureIntro; apply dom_fmap_L|].
-        iSplitL; first admit. (* this clearly holds *)
+        iSplitL.
+        { admit. (* this clearly holds *) }
         iIntros (r w HrPC Hr).
         rewrite lookup_fmap_Some in Hr.
         destruct Hr as (? & <- & Hr').
@@ -499,18 +591,32 @@ Section fundamental.
       all: cbn in HcorrectWret.
       all: inversion HcorrectWret; simplify_eq.
       + (* wret was a regular capability: apply the IH *)
-        iApply ("IH" with "[] [] [$] [] [] [$Hsts] [$Hcont_K] [$Hna] [$Hcstk_frag] [$]").
+        iApply ("IH" with "[] [] [$] [] [Hr] [$Hsts] [$Hcont_K] [$Hna] [$Hcstk_frag] [$]").
         { admit. (* easy *) }
-        { admit. (* easy, expect proving that the stack is safe, which is fine because of the clearing *) }
+        {
+          iIntros (r rv HrPC Hr).
+          destruct (decide (r = csp)); simplify_map_eq.
+          { admit. (* doable, but tedious *) }
+          destruct (decide (r = cs1)); simplify_map_eq; first done.
+          destruct (decide (r = cs0)); simplify_map_eq; first done.
+          destruct (decide (r = ca1)); simplify_map_eq; first done.
+          destruct (decide (r = ca0)); simplify_map_eq; first done.
+          destruct (decide (r = cgp)); simplify_map_eq; first done.
+          destruct (decide (r = cra)); simplify_map_eq; first done.
+          iApply "Hrmap_interp'"; eauto.
+          iPureIntro.
+          rewrite lookup_delete_ne; eauto.
+        }
         { iPureIntro; simplify_map_eq; done. }
         { admit. (* just close the region *) }
 
       + (* wret was a sentry capability: apply the def of safe for sentry *)
-        iEval (rewrite fixpoint_interp1_eq /=) in "Hinterp_wret".
+        iAssert (interp W C (WSentry p g b e a)) as "#Hinterp_wret'" ; first done.
+        iEval (rewrite fixpoint_interp1_eq /=) in "Hinterp_wastk2".
         destruct ( is_switcher_entry_point p g b e a ) eqn:Hwret_is_switcher_entry_point.
         (* The caller had changed the `wret` into one of the switcher's entry point.... *)
         * admit. (* TODO I need an inductive case *)
-        * iDestruct "Hinterp_wret" as "#Hinterp_wret".
+        * iDestruct "Hinterp_wastk2" as "#Hinterp_wret".
           rewrite /enter_cond.
           iAssert (future_world g W W) as "-#Hfuture".
           { destruct g; cbn; iPureIntro
@@ -524,7 +630,19 @@ Section fundamental.
           iSplitR.
           { iSplit.
             - admit. (* easy *)
-            - admit. (* easy, expect proving that the stack is safe, which is fine because of the clearing *)
+            -
+              iIntros (r rv HrPC Hr).
+              destruct (decide (r = csp)); simplify_map_eq.
+              { admit. (* doable, but tedious *) }
+              destruct (decide (r = cs1)); simplify_map_eq; first done.
+              destruct (decide (r = cs0)); simplify_map_eq; first done.
+              destruct (decide (r = ca1)); simplify_map_eq; first done.
+              destruct (decide (r = ca0)); simplify_map_eq; first done.
+              destruct (decide (r = cgp)); simplify_map_eq; first done.
+              destruct (decide (r = cra)); simplify_map_eq; first done.
+              iApply "Hrmap_interp'"; eauto.
+              iPureIntro.
+              rewrite lookup_delete_ne; eauto.
           }
           iSplitR.
           { iPureIntro; simplify_map_eq; done. }
